theory/JITFlattern_def.thy
@@ -1,9 +1,9 @@
 theory JITFlattern_def
   imports x64Semantics
 begin
-type_synonym flat_bpf_prog = "x64_bin \<times> (int \<times> nat) list \<times> ((int\<times>u64) list)"
+type_synonym flat_bpf_prog = "x64_bin \<times> (nat \<times> nat) list \<times> ((int\<times>u64) list)"
 
-definition update_l_jump::"(nat \<times> u64 \<times> x64_bin) \<Rightarrow> (int \<times> nat) list \<Rightarrow> (int\<times>u64) list \<Rightarrow> (int\<times>u64) list" where
+definition update_l_jump::"(nat \<times> u64 \<times> x64_bin) \<Rightarrow> (nat \<times> nat) list \<Rightarrow> (int\<times>u64) list \<Rightarrow> (int\<times>u64) list" where
 "update_l_jump x l_pc l_jump \<equiv> let (num,off,l_bin0) = x in 
   case x64_decode 0 l_bin0 of 
   Some(_, Pcall_i _) \<Rightarrow> l_jump@ [(of_nat (length l_pc), off)]|
@@ -21,7 +21,7 @@ fun jitflat_bpf :: "(nat \<times> u64 \<times> x64_bin) list \<Rightarrow> flat_
         l_jump')
 )"
 
-definition init_second_layer::"x64_bin \<times> (int \<times> nat) list \<times> ((int\<times>u64) list)" where
+definition init_second_layer::"x64_bin \<times> (nat \<times> nat) list \<times> ((int\<times>u64) list)" where
 "init_second_layer \<equiv> ([],[],[])"
 
 (*fun well_formed_prog_aux::"(nat \<times> u64 \<times> x64_bin) list \<Rightarrow> bool" where
@@ -47,18 +47,18 @@ definition well_formed_prog::"(nat \<times> u64 \<times> x64_bin) list \<Rightar
 "well_formed_prog lt \<equiv> ( lt \<noteq> [] \<and> 
   (\<forall> id. id < length lt \<and> id \<ge>0 \<longrightarrow> snd(snd (lt!id)) \<noteq> [] \<and> fst(lt!id) >0))"
 
-fun find_target_pc_in_l_pc :: "((int\<times>u64) list) \<Rightarrow> int \<Rightarrow> u64 option" where
+fun find_target_pc_in_l_pc :: "((int\<times>u64) list) \<Rightarrow> nat \<Rightarrow> u64 option" where
 "find_target_pc_in_l_pc [] _ = None" |
 "find_target_pc_in_l_pc ((x, y)#xs) pc = (
-  if x = pc then Some y
+  if x = of_nat pc then Some y
   else find_target_pc_in_l_pc xs pc
 )"
 
 
-fun find_target_pc_in_l_pc3 :: "((int\<times>u64) list) \<Rightarrow> int \<Rightarrow> int option" where
+fun find_target_pc_in_l_pc3 :: "((int\<times>u64) list) \<Rightarrow> nat \<Rightarrow> int option" where
 "find_target_pc_in_l_pc3 [] _ = None" |
 "find_target_pc_in_l_pc3 ((x, y)#xs) pc = (
-  if y = (of_int pc) then Some x
+  if y = of_nat pc then Some x
   else find_target_pc_in_l_pc3 xs pc
 )"
 
@@ -120,13 +120,13 @@ definition flat_bpf_one_step :: "flat_bpf_prog \<Rightarrow> hybrid_state \<Righ
     Next xpc rs m ss \<Rightarrow> (
     if unat pc \<ge> length l_pc \<or> unat pc < 0 then (pc,Stuck) else 
     let num = snd (l_pc!(unat pc)) in 
-    let old_xpc = nat (fst (l_pc!(unat pc))) in 
+    let old_xpc = fst (l_pc!(unat pc)) in 
       if xpc \<noteq> old_xpc then (pc, Stuck) else 
         case x64_decode xpc l_bin of Some(sz, Pcall_i imm) \<Rightarrow>
-            (case find_target_pc_in_l_pc l_jump (uint pc) of 
+            (case find_target_pc_in_l_pc l_jump (unat pc) of 
               None \<Rightarrow> (pc, Stuck) |
               Some npc \<Rightarrow> (
-                let xst_temp = exec_instr (Pcall_i (of_int(fst (l_pc!(unat npc))))) sz xpc rs m ss in 
+                let xst_temp = exec_instr (Pcall_i (of_nat(fst (l_pc!(unat npc))))) sz xpc rs m ss in 
                   (case xst_temp of Stuck \<Rightarrow> (pc, Stuck) | 
                                     Next xpc' rs' m' ss' \<Rightarrow> (npc, (Next xpc' rs' m' ss'))))) |
         Some(sz,Pcmpq_rr src dst) \<Rightarrow> \<comment>\<open> TODO: if the first byte is the opcode of cmp? \<close>
@@ -135,11 +135,11 @@ definition flat_bpf_one_step :: "flat_bpf_prog \<Rightarrow> hybrid_state \<Righ
             (case x64_sem num l_bin (Next xpc rs m ss) of
             Stuck \<Rightarrow> (pc, Stuck) | \<comment>\<open> if one step error, stop, it should be impossible \<close>
             Next xpc1 rs1 m1 ss1 \<Rightarrow> (
-              case find_target_pc_in_l_pc l_jump (uint pc) of
+              case find_target_pc_in_l_pc l_jump (unat pc) of
                 None \<Rightarrow> (pc, Stuck) |
                 Some npc \<Rightarrow>
               if rs1 (CR ZF) = 1 then \<comment>\<open> must JUMP \<close>
-                ((npc, (Next (nat (fst (l_pc!(unat npc)))) rs1 m1 ss1))) \<comment>\<open> go to the target address in the jited x64 binary \<close>
+                ((npc, (Next (fst (l_pc!(unat npc))) rs1 m1 ss1))) \<comment>\<open> go to the target address in the jited x64 binary \<close>
               else \<comment>\<open> donot JUMP \<close>
                 (pc+1, (Next (xpc1+sz2) rs1 m1 ss1))
             ))|
@@ -147,11 +147,11 @@ definition flat_bpf_one_step :: "flat_bpf_prog \<Rightarrow> hybrid_state \<Righ
         Some(sz,Pret_anchor) \<Rightarrow>
           (case x64_decode (xpc+sz) l_bin of Some (sz2,Pret) \<Rightarrow>
           let (pc', ss', caller,fp) = update_stack2 ss in 
-          if find_target_pc_in_l_pc3 l_jump (uint pc) \<noteq> Some (uint pc') then (pc,Stuck) else
+          if find_target_pc_in_l_pc3 l_jump (unat pc) \<noteq> Some (uint pc') then (pc,Stuck) else
           let rs' = restore_x64_caller rs caller fp in 
           let xst_temp = exec_instr Pret sz2 (xpc+sz) rs' m ss' in 
           (case xst_temp of Stuck \<Rightarrow> (pc,Stuck)| Next xpc1 rs1 m1 ss1 \<Rightarrow> 
-            (if xpc1 = (nat (fst (l_pc!(unat pc')))+1) then (pc',Next xpc1 rs1 m1 ss1) else (pc,Stuck) ))|
+            (if xpc1 = (fst (l_pc! (unat pc')))+1 then (pc',Next xpc1 rs1 m1 ss1) else (pc,Stuck) ))|
           _ \<Rightarrow> (pc,Stuck)) |
           \<comment>\<open> case: NOT BPF JMP \<close>
         _ \<Rightarrow>
